Added threadinfo argument; proved mul63

c/int63.c
@@ -9,7 +9,6 @@
 
 /*
  * Encoding/decoding
- */
 value certicoq_encode_int63(int64_t x) {
     return (x << 1) | 1;
 }
@@ -17,11 +16,10 @@ value certicoq_encode_int63(int64_t x) {
 int64_t certicoq_decode_int63(value x) {
     return (int64_t)x >> 1;
 }
-
+*/
 
 /*
  * Prims
- */
 value certicoq_prim__int63_zero() {
     return certicoq_encode_int63(0);
 }
@@ -37,31 +35,34 @@ value certicoq_prim__int63_neg(value x) {
 value certicoq_prim__int63_abs(value x) {
     return x < 0 ? certicoq_prim__int63_neg(x) : x;
 }
+*/
 
-value certicoq_prim__int63_add(value x, value y) {
+value certicoq_prim__int63_from_Z(struct thread_info *tinfo, value x) {
+  return 0;  
+}
+
+value certicoq_prim__int63_to_Z(struct thread_info *tinfo, value x) {
+  size_t n = ((uintnat)x)>>1;
+  return 0;  
+}
+
+value certicoq_prim__int63_add(struct thread_info *tinfo, value x, value y) {
   return (value)(((uintnat)x + (uintnat)y) - (uintnat)1);
 }
 
-value certicoq_prim__int63_sub(value x, value y) {
+value certicoq_prim__int63_sub(struct thread_info *tinfo, value x, value y) {
     return (x - y) + 1;
 }
 
-value certicoq_prim__int63_mul(value x, value y) {
-  return (value)(((uintnat)x * (uintnat)y) - (uintnat)1);
-
-    const int64_t _x = certicoq_decode_int63(x);
-    const int64_t _y = certicoq_decode_int63(y);
-    const int64_t _z = _x * _y;
-    return certicoq_encode_int63(_z);
+value certicoq_prim__int63_mul(struct thread_info *tinfo, value x, value y) {
+  return (value)((((uintnat)x)>>1) * (((uintnat)y)-1) + 1);
 }
 
-value certicoq_prim__int63_div(value x, value y) {
-    const int64_t _x = certicoq_decode_int63(x);
-    const int64_t _y = certicoq_decode_int63(y);
-    const int64_t _z = _x / _y;
-    return certicoq_encode_int63(_z);
+value certicoq_prim__int63_div(struct thread_info *tinfo, value x, value y) {
+  return (value)((((uintnat)x)-1) * (((uintnat)y)>>1)+(uintnat)1);
 }
 
+/*
 value certicoq_prim__int63_rem(value x, value y) {
     const int64_t _x = certicoq_decode_int63(x);
     const int64_t _y = certicoq_decode_int63(y);
@@ -82,31 +83,33 @@ value certicoq_prim__int63_shiftr(value x, value y) {
     const int64_t _z = _x >> _y;
     return certicoq_encode_int63(_z);
 }
+*/
 
-value certicoq_prim__int63_or(value x, value y) {
+value certicoq_prim__int63_or(struct thread_info *tinfo, value x, value y) {
     return x | y;
 }
 
-value certicoq_prim__int63_and(value x, value y) {
+value certicoq_prim__int63_and(struct thread_info *tinfo, value x, value y) {
     return x & y;
 }
 
-value certicoq_prim__int63_xor(value x, value y) {
+value certicoq_prim__int63_xor(struct thread_info *tinfo, value x, value y) {
     return (value)1 | (x ^ y);
 }
 
-value certicoq_prim__int63_not(value x) {
+value certicoq_prim__int63_not(struct thread_info *tinfo, value x) {
     return (value)1 | ~ x;
 }
 
-value certicoq_prim__int63_is_eq(value x, value y) {
+value certicoq_prim__int63_is_eq(struct thread_info *tinfo, value x, value y) {
     return (x == y) ? make_Coq_Init_Datatypes_bool_true() : make_Coq_Init_Datatypes_bool_false();
 }
 
-value certicoq_prim__int63_is_lt(value x, value y) {
-    return (x < y) ? make_Coq_Init_Datatypes_bool_true() : make_Coq_Init_Datatypes_bool_false();
+value certicoq_prim__int63_is_lt(struct thread_info *tinfo, value x, value y) {
+  return ((uintnat)x < (uintnat)y) ? make_Coq_Init_Datatypes_bool_true() : make_Coq_Init_Datatypes_bool_false();
 }
 
+/*
 value certicoq_prim__int63_to_nat(struct thread_info *tinfo, value x_val) {
     int64_t x = certicoq_decode_int63(x_val);
     value ret = make_Coq_Init_Datatypes_nat_O();
@@ -116,5 +119,6 @@ value certicoq_prim__int63_to_nat(struct thread_info *tinfo, value x_val) {
     }
     return ret;
 }
+*/
 
 #endif /* CERTICOQ_INT63_C */
