c/int63.h
@@ -15,23 +15,23 @@ int64_t certicoq_decode_int63(value x);
 /*
  * Prims
  */
-value certicoq_prim__int63_zero();
-value certicoq_prim__int63_one();
-value certicoq_prim__int63_neg(value x);
-value certicoq_prim__int63_abs(value x);
-value certicoq_prim__int63_add(value x, value y);
-value certicoq_prim__int63_sub(value x, value y);
-value certicoq_prim__int63_mul(value x, value y);
-value certicoq_prim__int63_div(value x, value y);
-value certicoq_prim__int63_rem(value x, value y);
-value certicoq_prim__int63_shiftl(value x, value y);
-value certicoq_prim__int63_shiftr(value x, value y);
-value certicoq_prim__int63_or(value x, value y);
-value certicoq_prim__int63_and(value x, value y);
-value certicoq_prim__int63_xor(value x, value y);
-value certicoq_prim__int63_not(value x);
-value certicoq_prim__int63_is_eq(value x, value y);
-value certicoq_prim__int63_is_lt(value x, value y);
+value certicoq_prim__int63_zero(struct thread_info *tinfo);
+value certicoq_prim__int63_one(struct thread_info *tinfo);
+value certicoq_prim__int63_neg(struct thread_info *tinfo, value x);
+value certicoq_prim__int63_abs(struct thread_info *tinfo, value x);
+value certicoq_prim__int63_add(struct thread_info *tinfo, value x, value y);
+value certicoq_prim__int63_sub(struct thread_info *tinfo, value x, value y);
+value certicoq_prim__int63_mul(struct thread_info *tinfo, value x, value y);
+value certicoq_prim__int63_div(struct thread_info *tinfo, value x, value y);
+value certicoq_prim__int63_rem(struct thread_info *tinfo, value x, value y);
+value certicoq_prim__int63_shiftl(struct thread_info *tinfo, value x, value y);
+value certicoq_prim__int63_shiftr(struct thread_info *tinfo, value x, value y);
+value certicoq_prim__int63_or(struct thread_info *tinfo, value x, value y);
+value certicoq_prim__int63_and(struct thread_info *tinfo, value x, value y);
+value certicoq_prim__int63_xor(struct thread_info *tinfo, value x, value y);
+value certicoq_prim__int63_not(struct thread_info *tinfo, value x);
+value certicoq_prim__int63_is_eq(struct thread_info *tinfo, value x, value y);
+value certicoq_prim__int63_is_lt(struct thread_info *tinfo, value x, value y);
 value certicoq_prim__int63_to_nat(struct thread_info *tinfo, value x_val);
 
 #endif /* CERTICOQ_INT63_H */
