c/verif_int63.v
@@ -36,3 +36,38 @@ apply Zbits.eqmod_mod.
 lia.
 Qed.
 
+Lemma body_mul: semax_body Vprog ASI f_certicoq_prim__int63_mul certicoq_prim__int63_mul_spec.
+Proof.
+unfold certicoq_prim__int63_mul_spec, tag63.
+start_function.
+forward.
+apply prop_right.
+f_equal.
+destruct x as [a ?].
+destruct y as [b ?].
+simpl proj1_sig.
+unfold Int64.shru.
+rewrite !Int64.unsigned_repr by rep_lia.
+rewrite mul64_repr.
+rewrite Z.shiftr_div_pow2 by lia.
+rewrite add64_repr.
+rewrite Z.pow_1_r.
+replace ((2 * a + 1)/2) with a.
+2:{
+rewrite Z.add_comm.
+rewrite Z.mul_comm.
+rewrite Z.div_add by lia.
+simpl. lia.
+}
+rewrite Z.add_simpl_r.
+replace (a*(2*b)) with (2*(a*b)) by ring.
+forget (a+b) as c.
+clear.
+apply Int64.eqm_samerepr.
+apply Int64.eqm_add; [ | apply Int64.eqm_refl].
+unfold Int64.eqm.
+change Int64.modulus with (2 * 2^63).
+apply eqmod_mul_m.
+apply Zbits.eqmod_mod.
+lia.
+Qed.
